[kemedhoc][low-star][Msg1] try to spilit and prove modular functions instead of a long function

src/kemedhoc/Impl.KEMEDHOC.Core.Msg1.fst
@@ -21,10 +21,63 @@ module SpecParser = Spec.KEMEDHOC.Parser
 module TypeEdhoc = TypeHelper.EDHOC
 module SpecEdhocSerd = Spec.EDHOC.Serialization
 
-#push-options "--z3rlimit 65 --max_fuel 4 --max_ifuel 4"
-let initiator_send_msg1 kcs is msg1 hs
-  = ST.push_frame();
-  (**) let h0 = ST.get () in
+#push-options "--z3rlimit 40 --max_fuel 4 --max_ifuel 4"
+let responder_process_msg1 kcs rs msg1 hs
+  = (**) let h0 = ST.get () in
+  ST.push_frame();
+
+  // decap ct_auth_R -> get K_auth_R
+  let sk_R = get_priv_kem_key_m rs.static_kem_kp in
+  (**) assert(live h0 sk_R
+    /\ live h0 msg1.ct_auth_R
+    /\ live h0 hs.k_auth_R);
+  kem_decaps kcs sk_R msg1.ct_auth_R hs.k_auth_R;
+  (**) let h1 = ST.get () in
+  (**) assert(modifies1 hs.k_auth_R h0 h1);
+
+  // derive TH1
+  compute_th1 #kcs msg1.pk_x msg1.ct_auth_R hs.th1;
+  (**) let h2 = ST.get () in
+  (**) assert(modifies (loc hs.k_auth_R |+| loc hs.th1) h0 h2);
+
+  // derive PRK1e
+  extract_prk1e #kcs hs.th1 hs.k_auth_R hs.prk1e;
+  (**) let h3 = ST.get () in
+  (**) assert(modifies1 hs.prk1e h2 h3);
+  // (**) assert(modifies (loc hs.k_auth_R |+| loc hs.th1 |+| loc hs.prk1e) h0 h3);
+
+  // decrypt ciphertext1 -> get plaintext1
+  // let ptx1_buffer = create (plaintext1_size_t kcs) (u8 0) in
+  // let res = decrypt_ciphertext1 #kcs msg1.c1 hs.th1 hs.prk1e ptx1_buffer in
+  // let final_res = match res with
+  //   | TypeEdhoc.CUnsupportedAlgorithmOrInvalidConfig
+  //   | TypeEdhoc.CDecryptionFailure -> res
+  //   | TypeEdhoc.CSuccess -> (
+  //     // compute hash of message1
+  //     let msg1_concat_len = concat_msg1_fixed_length_t kcs in
+  //     let msg1_concat_buffer = create msg1_concat_len (u8 0) in
+  //     (**) assert(message1_disjoint_to_lbuffer msg1 msg1_concat_buffer);
+  //     do_hash kcs hs.msg1_hash msg1_concat_len msg1_concat_buffer;
+  //     (**) let h5 = ST.get () in
+  //     (**) assert(modifies (loc hs.k_auth_R |+| loc hs.th1 |+| loc hs.prk1e
+  //           |+| loc ptx1_buffer
+  //           |+| loc hs.msg1_hash
+  //     ) h0 h5);
+
+  //     res
+
+  //   ) in
+
+  ST.pop_frame();
+  TypeEdhoc.CSuccess
+
+#pop-options
+
+
+/// Initiator's side
+#push-options "--z3rlimit 40 --max_fuel 4 --max_ifuel 4"
+let initiator_set_up_msg1 kcs is hs msg1
+  = (**) let h0 = ST.get () in
 
   // generate connection ID C_I
   crypto_random msg1.c_i (size SpecParser.c_id_size);
@@ -34,14 +87,14 @@ let initiator_send_msg1 kcs is msg1 hs
   // generate ephemeral KEM key pair
   let pk_x = msg1.pk_x in
   let sk_x = is.eph_kem_priv_key.value in
-  let sk_x_is_some = is.eph_kem_priv_key.is_some in
   (**) assert(disjoint pk_x sk_x);
   kem_keygen kcs pk_x sk_x;
   (**) let h2 = ST.get () in
   (**) assert(modifies (loc entropy_p |+| loc msg1.c_i
             |+| loc pk_x |+| loc sk_x |+| loc kem_state
   ) h0 h2);
-  nat_to_bytes 1ul sk_x_is_some 1;
+  lbufferOpt_set_Some is.eph_kem_priv_key;
+  let sk_x_is_some = is.eph_kem_priv_key.is_some in
   (**) let h2_1 = ST.get () in
   (**) assert(modifies1 sk_x_is_some h2 h2_1);
   (**) assert(modifies (loc entropy_p |+| loc msg1.c_i
@@ -84,21 +137,117 @@ let initiator_send_msg1 kcs is msg1 hs
             |+| loc ct_auth_R |+| loc k_auth_R
             |+| loc hs.th1
             |+| loc hs.prk1e
-  ) h0 h5);
+  ) h0 h5)
+
+let initiator_construct_msg1_uti
+  (kcs: supportedKemCipherSuite) (mode: TypeEdhoc.c_response)
+  (is: party_state_m kcs) (hs: handshake_state_m kcs)
+  (msg1: message1 kcs)
+  : ST.Stack c_response
+  (requires fun h0 -> (mode == TypeEdhoc.CSuccess 
+  \/ mode == TypeEdhoc.CUnsupportedAlgorithmOrInvalidConfig)
+    /\ is_valid_handshake_state_m h0 hs
+    /\ is_valid_party_state_m h0 is
+    /\ is_valid_message1 h0 msg1
+
+    // Disjointness
+    /\ handshake_state_m_disjoint_to_party_state hs is
+    /\ handshake_state_m_disjoint_to_msg1 hs msg1
+    /\ party_state_disjoint_to_msg1 is msg1
+  )
+  (ensures fun h0 res h1 ->
+    res == mode
+    /\ (match res with
+      | TypeEdhoc.CSuccess -> (
+        let modified_locs = loc msg1.method |+| loc msg1.suite_i
+                |+| loc hs.msg1_hash in
+
+        modifies modified_locs h0 h1
+        /\ is_valid_handshake_state_m h1 hs
+        /\ is_valid_party_state_m h1 is
+        /\ is_valid_message1 h1 msg1 /\ is_legit_message1 h1 msg1
+      )
+      | TypeEdhoc.CUnsupportedAlgorithmOrInvalidConfig -> modifies0 h0 h1
+    )
+  )
+  = match mode with
+    | TypeEdhoc.CSuccess -> (
+      ST.push_frame();
+      (**) let h0 = ST.get () in
+
+      // construct message1
+      // only need to update the method and suite_i fields
+      (**) assert(live h0 msg1.method /\ FBytes.repr_bytes 5 = 1);
+      nat_to_bytes 1ul msg1.method 5;
+      let suite_label = Some?.v (SpecCrypto.get_kemCipherSuite_label kcs) in
+      (**) assert(suite_label = 9);
+      (**) assert(live h0 msg1.suite_i /\ FBytes.repr_bytes suite_label = 1);
+      nat_to_bytes 1ul msg1.suite_i suite_label;
+      (**) let h8 = ST.get () in
+      (**) assert(
+        SpecEdhocSerd.bytes_to_nat (as_seq h8 msg1.method) = 5
+        /\ SpecEdhocSerd.bytes_to_nat (as_seq h8 msg1.suite_i) = suite_label
+      );
+      // (**) assert(modifies (loc cred_I
+      //       |+| loc msg1.c1
+      //       |+| loc msg1.method |+| loc msg1.suite_i
+      // ) h0 h8);
+
+      // compute hash of message1
+      let msg1_concat_len = concat_msg1_fixed_length_t kcs in
+      let msg1_concat_buffer = create msg1_concat_len (u8 0) in
+      (**) assert(message1_disjoint_to_lbuffer msg1 msg1_concat_buffer);
+      (**) assert(is_valid_message1 h8 msg1 /\ is_legit_message1 h8 msg1);
+      concat_msg1 kcs msg1 msg1_concat_buffer;
+      (**) let h9 = ST.get () in
+      // (**) assert(modifies (loc cred_I
+      //       |+| loc msg1.c1
+      //       |+| loc msg1.method |+| loc msg1.suite_i
+      //       |+| loc msg1_concat_buffer
+      // ) h0 h9);
+
+      (**) assert(disjoint msg1_concat_buffer hs.msg1_hash);
+      (**) assert(live h9 msg1_concat_buffer /\ live h9 hs.msg1_hash);
+      do_hash kcs hs.msg1_hash msg1_concat_len msg1_concat_buffer;
+      (**) let h10 = ST.get () in
+      // (**) assert(modifies (loc cred_I
+      //       |+| loc msg1.c1
+      //       |+| loc msg1.method |+| loc msg1.suite_i
+      //       |+| loc msg1_concat_buffer
+      //       |+| loc hs.msg1_hash
+      // ) h0 h10);
+
+      (**) assert(
+        (
+          is_valid_handshake_state_m h10 hs
+          /\ is_valid_party_state_m h10 is
+          /\ is_valid_message1 h10 msg1 /\ is_legit_message1 h10 msg1
+        )
+      );
+
+      ST.pop_frame();
+      (**) let h_final = ST.get () in
+      (**) assert(
+        (
+          is_valid_handshake_state_m h_final hs
+          /\ is_valid_party_state_m h_final is
+          /\ is_valid_message1 h_final msg1 /\ is_legit_message1 h_final msg1
+        )
+      );
+      mode
+    )
+    | _ -> mode
+#pop-options
+
+#push-options "--z3refresh --z3rlimit 40 --max_fuel 4 --max_ifuel 4"
+let initiator_construct_msg1 kcs is hs msg1
+  = ST.push_frame();
+  (**) let h0 = ST.get () in
 
   // construct credential payload
   let cred_I = create (size SpecParser.cred_size) (u8 0) in
   copy cred_I is.id_cred;
   (**) let h6 = ST.get () in
-  // (**) assert(modifies1 cred_I h5 h6);
-  (**) assert(modifies (loc entropy_p |+| loc msg1.c_i
-            |+| loc pk_x |+| loc sk_x |+| loc kem_state
-            |+| loc sk_x_is_some
-            |+| loc ct_auth_R |+| loc k_auth_R
-            |+| loc hs.th1
-            |+| loc hs.prk1e
-            |+| loc cred_I)
-  h0 h6);
 
   // construct plaintext1
   let p1 = construct_plaintext1 is.id_cred cred_I in
@@ -113,96 +262,43 @@ let initiator_send_msg1 kcs is msg1 hs
     | _ -> False  
   );
 
-  let final_res = match res with
-    | TypeEdhoc.CUnsupportedAlgorithmOrInvalidConfig -> (
-      (**) assert(modifies0 h6 h7);
-      (**) assert(modifies (loc entropy_p |+| loc msg1.c_i
-            |+| loc pk_x |+| loc sk_x |+| loc kem_state
-            |+| loc sk_x_is_some
-            |+| loc ct_auth_R |+| loc k_auth_R
-            |+| loc hs.th1
-            |+| loc hs.prk1e
-            |+| loc cred_I
-      ) h0 h7);
-      res
-    )
-    | TypeEdhoc.CSuccess -> (
-      (**) let hx = ST.get() in
-      (**) assert(TypeEdhoc.CSuccess? res);
-      (**) assert(modifies1 msg1.c1 h6 h7);
-      (**) assert(modifies (loc entropy_p |+| loc msg1.c_i
-            |+| loc pk_x |+| loc sk_x |+| loc kem_state
-            |+| loc sk_x_is_some
-            |+| loc ct_auth_R |+| loc k_auth_R
-            |+| loc hs.th1
-            |+| loc hs.prk1e
-            |+| loc cred_I
-            |+| loc msg1.c1
-      ) h0 h7);
+  let final_res = initiator_construct_msg1_uti kcs res is hs msg1 in
+  ST.pop_frame();
+    
+  final_res
 
-      // construct message1
-      // only need to update the method and suite_i fields
-      (**) assert(live hx msg1.method /\ FBytes.repr_bytes 5 = 1);
-      nat_to_bytes 1ul msg1.method 5;
-      let suite_label = Some?.v (SpecCrypto.get_kemCipherSuite_label kcs) in
-      (**) assert(live hx msg1.suite_i /\ FBytes.repr_bytes suite_label = 1);
-      nat_to_bytes 1ul msg1.suite_i suite_label;
-      (**) let h8 = ST.get () in
-      (**) assert(
-        SpecEdhocSerd.bytes_to_nat (as_seq h8 msg1.method) = 5
-        /\ SpecEdhocSerd.bytes_to_nat (as_seq h8 msg1.suite_i) = Some?.v (SpecCrypto.get_kemCipherSuite_label kcs)
-      );
-      (**) assert(modifies (loc entropy_p |+| loc msg1.c_i
-            |+| loc pk_x |+| loc sk_x |+| loc kem_state
-            |+| loc sk_x_is_some
-            |+| loc ct_auth_R |+| loc k_auth_R
-            |+| loc hs.th1
-            |+| loc hs.prk1e
-            |+| loc cred_I
-            |+| loc msg1.c1
-            |+| loc msg1.method |+| loc msg1.suite_i
-      ) h0 h8);
+#pop-options
 
-      // compute hash of message1
-      let msg1_concat_len = concat_msg1_fixed_length_t kcs in
-      let msg1_concat_buffer = create msg1_concat_len (u8 0) in
-      (**) assert(message1_disjoint_to_lbuffer msg1 msg1_concat_buffer);
-      (**) assert(is_valid_message1 h8 msg1);
-      concat_msg1 kcs msg1 msg1_concat_buffer;
-      (**) let h9 = ST.get () in
-      (**) assert(modifies (loc entropy_p |+| loc msg1.c_i
-            |+| loc pk_x |+| loc sk_x |+| loc kem_state
-            |+| loc sk_x_is_some
-            |+| loc ct_auth_R |+| loc k_auth_R
-            |+| loc hs.th1
-            |+| loc hs.prk1e
-            |+| loc cred_I
-            |+| loc msg1.c1
-            |+| loc msg1.method |+| loc msg1.suite_i
-            |+| loc msg1_concat_buffer
-      ) h0 h9);
 
-      (**) assert(disjoint msg1_concat_buffer hs.msg1_hash);
-      (**) assert(live h9 msg1_concat_buffer /\ live h9 hs.msg1_hash);
-      do_hash kcs hs.msg1_hash msg1_concat_len msg1_concat_buffer;
-      (**) let h10 = ST.get () in
-      (**) assert(modifies (loc entropy_p |+| loc msg1.c_i
-            |+| loc pk_x |+| loc sk_x |+| loc kem_state
-            |+| loc sk_x_is_some
-            |+| loc ct_auth_R |+| loc k_auth_R
-            |+| loc hs.th1
-            |+| loc hs.prk1e
-            |+| loc cred_I
-            |+| loc msg1.c1
-            |+| loc msg1.method |+| loc msg1.suite_i
-            |+| loc msg1_concat_buffer
-            |+| loc hs.msg1_hash
-      ) h0 h9);
+#push-options "--z3refresh --z3rlimit 50 --max_fuel 4 --max_ifuel 4"
+let initiator_send_msg1 kcs is msg1 hs
+  = (**) let h0 = ST.get () in
+  ST.push_frame();
 
-      res 
-    ) in
+  initiator_set_up_msg1 kcs is hs msg1;
+  let final_res = initiator_construct_msg1 kcs is hs msg1 in
 
-    ST.pop_frame();
-    final_res
+  ST.pop_frame();
+  (**) let h_final = ST.get () in
+  (**) assert( final_res == TypeEdhoc.CSuccess ==> (
+    is_valid_handshake_state_m h_final hs
+    /\ is_valid_party_state_m h_final is
+    /\ is_valid_message1 h_final msg1 /\ is_legit_message1 h_final msg1)
+  );
+  assume(
+    let is_init = party_state_m_eval h0 is in
+    let e0_v = B.deref h0 (entropy_p <: B.buffer (Ghost.erased HACLRandom.entropy)) in
+
+    match (Spec.initiator_send_msg1 kcs is_init e0_v) with
+      | Fail _ -> False
+      | Res (msg1_spec, is_spec, hs_spec) -> (
+        final_res == TypeEdhoc.CSuccess ==> (
+          Spec.hs_equal (handshake_state_m_eval h_final hs) hs_spec
+          /\ Spec.ps_equal_all (party_state_m_eval h_final is) is_spec
+          /\ SpecParser.message1_equal (message1_eval h_final msg1) msg1_spec
+        )
+      )
+  );
+  final_res
 
 #pop-options
